cedar-lean/Cedar/Data/Set.lean
@@ -14,9 +14,12 @@
  limitations under the License.
 -/
 
-import Cedar.Data.List
+module
+
+public import Cedar.Data.List
 import Batteries.Data.List.Basic
 import Batteries.Data.List.Lemmas
+public import Lean.Data.Json.FromToJson.Basic
 
 /-!
 # Canonical list-based sets
@@ -31,13 +34,13 @@ Use `Set.make` to construct well-formed sets from lists.
 
 namespace Cedar.Data
 
-inductive Set (α : Type u) where
+public inductive Set (α : Type u) where
 | mk (l : List α)
 deriving Repr, DecidableEq, Inhabited, Lean.ToJson
 
 namespace Set
 
-abbrev elts {α : Type u} (s : Set α) := s.1
+public abbrev elts {α : Type u} (s : Set α) := s.1
 
 ----- Definitions -----
 
@@ -45,113 +48,114 @@ abbrev elts {α : Type u} (s : Set α) := s.1
   Creates an ordered/duplicate free list from a set provided the underlying
   set is well formed.
 -/
-def toList {α : Type u} (s : Set α) : List α := s.elts
+@[expose]
+public def toList {α : Type u} (s : Set α) : List α := s.elts
 
 /-- Creates a well-formed set from the given list. -/
-def make [LT α] [DecidableLT α] (elts : List α) : Set α :=
+public def make [LT α] [DecidableLT α] (elts : List α) : Set α :=
   Set.mk (elts.canonicalize (·))
 
 /-- Empty set ∅ -/
-def empty {α} : Set α := .mk []
+public def empty {α} : Set α := .mk []
 
 /-- s == ∅ -/
-def isEmpty {α} [DecidableEq α] (s : Set α) : Bool :=
+public def isEmpty {α} [DecidableEq α] (s : Set α) : Bool :=
   s == empty
 
 /-- elt ∈ s -/
-def contains {α} [DecidableEq α] (s : Set α) (elt : α) : Bool :=
+public def contains {α} [DecidableEq α] (s : Set α) (elt : α) : Bool :=
   s.elts.elem elt                    -- can use binary search instead
 
 /-- s₁ ⊆ s₂ -/
-def subset {α} [DecidableEq α] (s₁ s₂ : Set α) : Bool :=
+public def subset {α} [DecidableEq α] (s₁ s₂ : Set α) : Bool :=
   s₁.elts.all s₂.contains
 
 /-- s₁ ∩ s₂ ≠ ∅ -/
-def intersects {α} [DecidableEq α] (s₁ s₂ : Set α) : Bool :=
+public def intersects {α} [DecidableEq α] (s₁ s₂ : Set α) : Bool :=
   s₁.elts.any s₂.contains
 
 /-- s₁ ∩ s₂ -/
-def intersect {α} [DecidableEq α] (s₁ s₂ : Set α) : Set α :=
+public def intersect {α} [DecidableEq α] (s₁ s₂ : Set α) : Set α :=
   Set.mk (s₁.elts.inter s₂.elts)      -- well-formed by construction
 
 /-- s₁ ∪ s₂ -/
-def union {α} [LT α] [DecidableLT α] (s₁ s₂ : Set α) : Set α :=
+public def union {α} [LT α] [DecidableLT α] (s₁ s₂ : Set α) : Set α :=
   make (s₁.elts ++ s₂.elts)           -- enforce well-formedness
 
-instance [LT α] [DecidableLT α] : HAppend (Set α) (Set α) (Set α) where
+public instance [LT α] [DecidableLT α] : HAppend (Set α) (Set α) (Set α) where
   hAppend := Set.union
 
 /-- Filters `s` using `f`. -/
-def filter {α} (f : α → Bool) (s : Set α) : Set α :=
+public def filter {α} (f : α → Bool) (s : Set α) : Set α :=
   Set.mk (s.elts.filter f)            -- well-formed by construction
 
 /-- s₁ \ s₂. -/
-def difference {α} [LT α] [DecidableLT α] [DecidableEq α] (s₁ s₂ : Set α) : Set α :=
+public def difference {α} [LT α] [DecidableLT α] [DecidableEq α] (s₁ s₂ : Set α) : Set α :=
   s₁.filter (!s₂.contains ·)
 
 /-- Maps `f` to `s`.-/
-def map {α β} [LT β] [DecidableLT β] (f : α → β) (s : Set α) : Set β :=
+public def map {α β} [LT β] [DecidableLT β] (f : α → β) (s : Set α) : Set β :=
   make (s.elts.map f)                 -- enforce well-formedness
 
 /-- Maps `f` to `s` and returns the result of `err` if any error is encountered. -/
-def mapOrErr {α β ε} [DecidableEq β] [LT β] [DecidableRel (α := β) (· < ·)] (f : α → Except ε β) (s : Set α) (err : ε) : Except ε (Set β) :=
+public def mapOrErr {α β ε} [DecidableEq β] [LT β] [DecidableRel (α := β) (· < ·)] (f : α → Except ε β) (s : Set α) (err : ε) : Except ε (Set β) :=
   match s.elts.mapM f with
   | .ok elts => .ok (make elts)    -- enforce well-formedness
   | .error _ => .error err         -- return fixed error to be order-independent
 
 /-- Returns true if all elements of `s` satisfy `f`. -/
-def all {α} (f : α → Bool) (s : Set α) : Bool :=
+public def all {α} (f : α → Bool) (s : Set α) : Bool :=
   s.elts.all f
 
 /-- Returns true if some element of `s` satisfies `f`. -/
-def any {α} (f : α → Bool) (s : Set α) : Bool :=
+public def any {α} (f : α → Bool) (s : Set α) : Bool :=
   s.elts.any f
 
-def size {α} (s : Set α) : Nat :=
+public def size {α} (s : Set α) : Nat :=
   s.elts.length
 
-def singleton {α} (a : α) : Set α :=
+public def singleton {α} (a : α) : Set α :=
   Set.mk [a]
 
 /-- Checks if a set if well-formed -/
-def wellFormed {α} [LT α] [DecidableLT α] (s : Set α) : Bool :=
+public def wellFormed {α} [LT α] [DecidableLT α] (s : Set α) : Bool :=
   s.elts.isSorted
 
 /-- If `s` is a singleton set, returns the single element -/
-def singleton? [Inhabited α] (s : Set α) : Option α :=
+public def singleton? [Inhabited α] (s : Set α) : Option α :=
   match s.elts with
   | [] => none
   | [x] => x
   | _ => none
 
-def foldl {α β} (f : α → β → α) (init : α) (s : Set β) : α :=
+public def foldl {α β} (f : α → β → α) (init : α) (s : Set β) : α :=
   s.elts.foldl f init
 
 ----- Instances -----
 
-instance [LT α] : LT (Set α) where
+public instance [LT α] : LT (Set α) where
   lt a b := a.elts < b.elts
 
-instance decLt [LT α] [DecidableEq α] [DecidableLT α] : (n m : Set α) → Decidable (n < m)
+public instance decLt [LT α] [DecidableEq α] [DecidableLT α] : (n m : Set α) → Decidable (n < m)
   | .mk nelts, .mk melts => List.decidableLT nelts melts
 
 -- enables ∅
-instance : EmptyCollection (Set α) where
+public instance : EmptyCollection (Set α) where
   emptyCollection := Set.empty
 
 -- enables ∈
-instance : Membership α (Set α) where
+public instance : Membership α (Set α) where
   mem s v := v ∈ s.elts
 
 -- enables ⊆
-instance [DecidableEq α] : HasSubset (Set α) where
+public instance [DecidableEq α] : HasSubset (Set α) where
   Subset s₁ s₂ := s₁.subset s₂
 
 -- enables ∩
-instance [DecidableEq α] : Inter (Set α) := ⟨Set.intersect⟩
+public instance [DecidableEq α] : Inter (Set α) := ⟨Set.intersect⟩
 
 -- enables ∪
-instance [LT α] [DecidableLT α] : Union (Set α) := ⟨Set.union⟩
+public instance [LT α] [DecidableLT α] : Union (Set α) := ⟨Set.union⟩
 
 end Set
 
