cedar-lean/Cedar/Thm/Data/Set.lean
@@ -14,9 +14,13 @@
  limitations under the License.
 -/
 
-import Cedar.Data.Set
+module
+
+public import Cedar.Data.Set
+import all Cedar.Data.Set -- inside this module, we're allowed to unfold defs in Cedar.Data.Set that are not normally exposed
 import Cedar.Thm.Data.Control
-import Cedar.Thm.Data.List
+public import Cedar.Thm.Data.List
+public import Cedar.Data.LT
 
 /-!
 # Set properties
@@ -29,16 +33,16 @@ namespace Cedar.Data.Set
 
 /-! ### Well-formed sets -/
 
-def WellFormed {α} [LT α] [DecidableLT α] (s : Set α) :=
+public def WellFormed {α} [LT α] [DecidableLT α] (s : Set α) :=
   s = Set.make s.toList
 
-theorem if_wellformed_then_exists_make [LT α] [DecidableLT α] (s : Set α) :
+public theorem if_wellformed_then_exists_make [LT α] [DecidableLT α] (s : Set α) :
   WellFormed s → ∃ list, s = Set.make list
 := by
   intro h₁
   exists s.elts
 
-theorem wf_iff_sorted {α} [LT α] [DecidableLT α] [StrictLT α]  (s : Set α) :
+public theorem wf_iff_sorted {α} [LT α] [DecidableLT α] [StrictLT α]  (s : Set α) :
   s.WellFormed ↔ s.elts.Sorted
 := by
   simp only [WellFormed, make, toList, elts]
@@ -56,14 +60,14 @@ theorem wf_iff_sorted {α} [LT α] [DecidableLT α] [StrictLT α]  (s : Set α) 
 
 /-! ### contains and mem -/
 
-theorem contains_prop_bool_equiv [DecidableEq α] {v : α} {s : Set α} :
+public theorem contains_prop_bool_equiv [DecidableEq α] {v : α} {s : Set α} :
   s.contains v = true ↔ v ∈ s
 := by
   constructor <;> intro h
   · exact List.mem_of_elem_eq_true h
   · exact List.elem_eq_true_of_mem h
 
-theorem not_contains_prop_bool_equiv [DecidableEq α] {v : α} {s : Set α} :
+public theorem not_contains_prop_bool_equiv [DecidableEq α] {v : α} {s : Set α} :
   s.contains v = false ↔ v ∉ s
 := by
   constructor
@@ -78,38 +82,38 @@ theorem not_contains_prop_bool_equiv [DecidableEq α] {v : α} {s : Set α} :
     | false =>
       rfl
 
-theorem in_list_iff_in_set {α : Type u} (v : α) (s : Set α) :
+public theorem in_list_iff_in_set {α : Type u} (v : α) (s : Set α) :
   v ∈ s.elts ↔ v ∈ s
 := by
   constructor
   case mp => intro h ; apply h
   case mpr => simp [elts, Membership.mem]
 
-theorem in_list_iff_in_mk {α : Type u} (v : α) (xs : List α) :
+public theorem in_list_iff_in_mk {α : Type u} (v : α) (xs : List α) :
   v ∈ xs ↔ v ∈ mk xs
 := by
   constructor
   case mp => intro h ; apply h
   case mpr => simp [elts, Membership.mem]
 
-theorem mem_cons_self {α : Type u} (hd : α) (tl : List α) :
+public theorem mem_cons_self {α : Type u} (hd : α) (tl : List α) :
   hd ∈ Set.mk (hd :: tl)
 := by
   simp only [Membership.mem, elts]
   exact List.mem_cons_self
 
-theorem mem_cons_of_mem {α : Type u} (a : α) (hd : α) (tl : List α) :
+public theorem mem_cons_of_mem {α : Type u} (a : α) (hd : α) (tl : List α) :
   a ∈ Set.mk tl → a ∈ Set.mk (hd :: tl)
 := by
   simp only [Membership.mem] ; intro h₁
   apply List.mem_cons_of_mem hd h₁
 
-theorem mem_cons {a : α} {hd : α} {tl : List α} :
+public theorem mem_cons {a : α} {hd : α} {tl : List α} :
   a ∈ Set.mk (hd :: tl) ↔ a = hd ∨ a ∈ tl
 := by
   simp [← in_list_iff_in_mk]
 
-theorem in_set_means_list_non_empty {α : Type u} (v : α) (s : Set α) :
+public theorem in_set_means_list_non_empty {α : Type u} (v : α) (s : Set α) :
   v ∈ s.elts → ¬(s.elts = [])
 := by
   intros h0 h1
@@ -119,11 +123,11 @@ theorem in_set_means_list_non_empty {α : Type u} (v : α) (s : Set α) :
 
 /-! ### empty -/
 
-theorem empty_eq_mk_empty {α} :
+public theorem empty_eq_mk_empty {α} :
   (Set.empty : Set α) = Set.mk []
 := by simp only [empty]
 
-theorem empty_no_elts {α : Type u} (v : α) :
+public theorem empty_no_elts {α : Type u} (v : α) :
   ¬ v ∈ Set.empty
 := by
   intro h
@@ -131,13 +135,13 @@ theorem empty_no_elts {α : Type u} (v : α) :
   have _ := List.ne_nil_of_mem h
   contradiction
 
-theorem empty_wf {α : Type u} [LT α] [DecidableLT α] :
+public theorem empty_wf {α : Type u} [LT α] [DecidableLT α] :
   Set.WellFormed (Set.empty : Set α)
 := by
-  unfold WellFormed toList empty make List.canonicalize
-  rfl
+  simp [WellFormed, toList, empty, make, elts]
+  apply List.canonicalize_nil
 
-theorem map_empty [LT β] [DecidableLT β] (f : α → β) :
+public theorem map_empty [LT β] [DecidableLT β] (f : α → β) :
   Set.empty.map f = Set.empty
 := by
   simp [Set.map, empty_eq_mk_empty, Set.elts, Set.make, List.canonicalize_nil]
@@ -145,7 +149,7 @@ theorem map_empty [LT β] [DecidableLT β] (f : α → β) :
 
 /-! ### isEmpty -/
 
-theorem make_empty [DecidableEq α] [LT α] [DecidableLT α] (xs : List α) :
+public theorem make_empty [DecidableEq α] [LT α] [DecidableLT α] (xs : List α) :
   xs = [] ↔ (Set.make xs).isEmpty
 := by
   unfold isEmpty; unfold empty; unfold make
@@ -159,14 +163,14 @@ theorem make_empty [DecidableEq α] [LT α] [DecidableLT α] (xs : List α) :
     apply (List.canonicalize_nil' id xs).mpr
     assumption
 
-theorem make_non_empty [DecidableEq α] [LT α] [DecidableLT α] (xs : List α) :
+public theorem make_non_empty [DecidableEq α] [LT α] [DecidableLT α] (xs : List α) :
   xs ≠ [] ↔ (Set.make xs).isEmpty = false
 := by
   unfold isEmpty; unfold empty; unfold make
   simp only [beq_eq_false_iff_ne, ne_eq, mk.injEq]
   apply List.canonicalize_not_nil
 
-theorem non_empty_iff_exists [DecidableEq α] (s : Set α) :
+public theorem non_empty_iff_exists [DecidableEq α] (s : Set α) :
   ¬ s.isEmpty ↔ ∃ a, a ∈ s
 := by
   simp only [isEmpty, empty, beq_iff_eq]
@@ -189,7 +193,7 @@ theorem non_empty_iff_exists [DecidableEq α] (s : Set α) :
     subst h₂
     simp [elts] at h₁
 
-theorem empty_iff_not_exists [DecidableEq α] (s : Set α) :
+public theorem empty_iff_not_exists [DecidableEq α] (s : Set α) :
   s.isEmpty ↔ ¬ ∃ a, a ∈ s
 := by
   simp only [isEmpty, empty, beq_iff_eq, not_exists]
@@ -212,28 +216,29 @@ theorem empty_iff_not_exists [DecidableEq α] (s : Set α) :
 
 /-! ### singleton -/
 
-theorem singleton_wf [DecidableEq α] [LT α] [DecidableLT α] (a : α) :
+public theorem singleton_wf [DecidableEq α] [LT α] [DecidableLT α] (a : α) :
   WellFormed (Set.singleton a)
 := by
-  simp [singleton, WellFormed, make, toList, List.canonicalize, List.insertCanonical_singleton]
+  simp [singleton, WellFormed, make, toList, elts]
+  rw [List.canonicalize_singleton]
 
-theorem mem_singleton_iff_eq [DecidableEq α] (a b : α) :
+public theorem mem_singleton_iff_eq [DecidableEq α] (a b : α) :
   a ∈ Set.singleton b ↔ a = b
 := by
   simp only [singleton, ← in_list_iff_in_mk, List.mem_singleton]
 
-theorem mem_singleton [DecidableEq α] (a : α) :
+public theorem mem_singleton [DecidableEq α] (a : α) :
   a ∈ Set.singleton a
 := by simp only [mem_singleton_iff_eq]
 
 /-! ### make -/
 
-theorem make_wf [LT α] [DecidableLT α] [StrictLT α] (xs : List α) :
+public theorem make_wf [LT α] [DecidableLT α] [StrictLT α] (xs : List α) :
   WellFormed (Set.make xs)
 := by
   simp only [WellFormed, make, toList, elts, List.canonicalize_idempotent]
 
-theorem make_sorted {α} [LT α] [DecidableLT α] [StrictLT α] {xs : List α} :
+public theorem make_sorted {α} [LT α] [DecidableLT α] [StrictLT α] {xs : List α} :
   xs.Sorted → Set.make xs = Set.mk xs
 := by
   intro h
@@ -241,7 +246,7 @@ theorem make_sorted {α} [LT α] [DecidableLT α] [StrictLT α] {xs : List α} :
     apply funext ; simp only [id_eq, implies_true]
   simp only [make, hid, List.sortedBy_implies_canonicalize_eq h]
 
-theorem make_mem [LT α] [DecidableLT α] [StrictLT α] (x : α) (xs : List α) :
+public theorem make_mem [LT α] [DecidableLT α] [StrictLT α] (x : α) (xs : List α) :
   x ∈ xs ↔ x ∈ Set.make xs
 := by
   simp only [make, Membership.mem]
@@ -252,7 +257,7 @@ theorem make_mem [LT α] [DecidableLT α] [StrictLT α] (x : α) (xs : List α) 
   case mp => exact h₁ h₃
   case mpr => exact h₂ h₃
 
-theorem make_mk_eqv [LT α] [DecidableLT α] [StrictLT α] {xs ys : List α} :
+public theorem make_mk_eqv [LT α] [DecidableLT α] [StrictLT α] {xs ys : List α} :
   Set.make xs = Set.mk ys → xs ≡ ys
 := by
   simp only [make, mk.injEq] ; intro h₁
@@ -260,7 +265,7 @@ theorem make_mk_eqv [LT α] [DecidableLT α] [StrictLT α] {xs ys : List α} :
   subst h₁
   exact h₂
 
-theorem make_make_eqv [LT α] [DecidableLT α] [StrictLT α] {xs ys : List α} :
+public theorem make_make_eqv [LT α] [DecidableLT α] [StrictLT α] {xs ys : List α} :
   Set.make xs = Set.make ys ↔ xs ≡ ys
 := by
   constructor <;> intro h
@@ -276,7 +281,7 @@ theorem make_make_eqv [LT α] [DecidableLT α] [StrictLT α] {xs ys : List α} :
     simp only [make, mk.injEq]
     apply List.equiv_implies_canonical_eq _ _ h
 
-theorem elts_make_equiv [LT α] [DecidableLT α] [StrictLT α] {xs : List α} :
+public theorem elts_make_equiv [LT α] [DecidableLT α] [StrictLT α] {xs : List α} :
   Set.elts (Set.make xs) ≡ xs
 := by
   simp only [List.Equiv, List.subset_def]
@@ -286,22 +291,22 @@ theorem elts_make_equiv [LT α] [DecidableLT α] [StrictLT α] {xs : List α} :
   · rw [in_list_iff_in_set, ← make_mem]
     exact h₁
 
-theorem make_nil [LT α] [DecidableLT α] [StrictLT α] :
+public theorem make_nil [LT α] [DecidableLT α] [StrictLT α] :
   Set.make [] (α := α) = Set.empty
 := by
   simp [make, List.canonicalize_nil, empty]
 
-theorem elts_make_nil [LT α] [DecidableLT α] [StrictLT α] :
+public theorem elts_make_nil [LT α] [DecidableLT α] [StrictLT α] :
   Set.elts (Set.make ([] : List α)) = []
 := by
   simp [make, elts, List.canonicalize_nil]
 
-theorem make_singleton_nonempty [LT α] [DecidableLT α] [StrictLT α] [DecidableEq α] (a : α) :
+public theorem make_singleton_nonempty [LT α] [DecidableLT α] [StrictLT α] [DecidableEq α] (a : α) :
   Set.make [a] ≠ Set.empty
 := by
-  simp [make, empty, List.canonicalize, List.insertCanonical_not_nil _ a []]
+  simp [make, empty, List.canonicalize_singleton]
 
-def eq_means_eqv [LT α] [DecidableLT α] [StrictLT α] {s₁ s₂ : Set α} :
+public def eq_means_eqv [LT α] [DecidableLT α] [StrictLT α] {s₁ s₂ : Set α} :
   WellFormed s₁ → WellFormed s₂ →
   (s₁.elts ≡ s₂.elts ↔ s₁ = s₂)
 := by
@@ -321,7 +326,7 @@ def eq_means_eqv [LT α] [DecidableLT α] [StrictLT α] {s₁ s₂ : Set α} :
     subst h₃
     apply List.Equiv.refl
 
-theorem make_any_iff_any [LT α] [DecidableLT α] [StrictLT α] (f : α → Bool) (xs : List α) :
+public theorem make_any_iff_any [LT α] [DecidableLT α] [StrictLT α] (f : α → Bool) (xs : List α) :
   (Set.make xs).any f = xs.any f
 := by
   simp only [make, any]
@@ -330,7 +335,7 @@ theorem make_any_iff_any [LT α] [DecidableLT α] [StrictLT α] (f : α → Bool
   have ⟨hl₁, hr₁⟩ := h₁
   cases h₃ : List.any xs f
   case false =>
-    by_contra h₄
+    false_or_by_contra ; rename_i h₄
     simp only [Bool.not_eq_false, List.any_eq_true] at h₄
     have ⟨x, h₄, h₅⟩ := h₄
     specialize hr₁ h₄
@@ -342,7 +347,7 @@ theorem make_any_iff_any [LT α] [DecidableLT α] [StrictLT α] (f : α → Bool
     simp only [h₄, and_true]
     apply hl₁ h₃
 
-theorem make_of_make_is_id [LT α] [DecidableLT α] [StrictLT α] (xs : List α) :
+public theorem make_of_make_is_id [LT α] [DecidableLT α] [StrictLT α] (xs : List α) :
   Set.make (Set.elts (Set.make xs)) = Set.make xs
 := by
   simp only [make, mk.injEq]
@@ -350,7 +355,7 @@ theorem make_of_make_is_id [LT α] [DecidableLT α] [StrictLT α] (xs : List α)
   unfold id at h₁
   exact h₁
 
-theorem elts_make_is_id_then_equiv [LT α] [DecidableLT α] [StrictLT α] {xs ys : List α} :
+public theorem elts_make_is_id_then_equiv [LT α] [DecidableLT α] [StrictLT α] {xs ys : List α} :
   Set.elts (Set.make xs) = ys → ys ≡ xs
 := by
   intro h
@@ -362,7 +367,7 @@ theorem elts_make_is_id_then_equiv [LT α] [DecidableLT α] [StrictLT α] {xs ys
   Note that the converse of this is not true:
   counterexample `xs = [1]`, `ys = []`, `a = 1`.
 -/
-theorem make_cons [LT α] [DecidableLT α] {xs ys : List α} {a : α} :
+public theorem make_cons [LT α] [DecidableLT α] {xs ys : List α} {a : α} :
   make xs = make ys → make (a :: xs) = make (a :: ys)
 := by
   simp only [make, mk.injEq]
@@ -370,12 +375,12 @@ theorem make_cons [LT α] [DecidableLT α] {xs ys : List α} {a : α} :
 
 /-! ### inter and union -/
 
-theorem inter_def {α} [LT α] [StrictLT α] [DecidableLT α] [DecidableEq α] {s₁ s₂ : Set α} :
+public theorem inter_def {α} [LT α] [StrictLT α] [DecidableLT α] [DecidableEq α] {s₁ s₂ : Set α} :
   s₁ ∩ s₂ = s₁.intersect s₂
 := by simp only [Inter.inter]
 
 open BEq LawfulBEq in
-theorem mem_inter_iff {α} [DecidableEq α] {x : α} {s₁ s₂ : Set α} :
+public theorem mem_inter_iff {α} [DecidableEq α] {x : α} {s₁ s₂ : Set α} :
   x ∈ s₁ ∩ s₂ ↔ x ∈ s₁ ∧ x ∈ s₂
 := by
   simp only [Membership.mem]
@@ -383,7 +388,7 @@ theorem mem_inter_iff {α} [DecidableEq α] {x : α} {s₁ s₂ : Set α} :
   simp only [Membership.mem, Inter.inter] at h
   exact h
 
-theorem inter_wf {α} [LT α] [StrictLT α] [DecidableLT α] [DecidableEq α] {s₁ s₂ : Set α}
+public theorem inter_wf {α} [LT α] [StrictLT α] [DecidableLT α] [DecidableEq α] {s₁ s₂ : Set α}
  (h₁ : WellFormed s₁) :
  WellFormed (s₁ ∩ s₂)
 := by
@@ -397,20 +402,20 @@ theorem inter_wf {α} [LT α] [StrictLT α] [DecidableLT α] [DecidableEq α] {s
   simp only [List.elem_eq_mem]
   exact h₃
 
-theorem inter_empty_left {α} [LT α] [StrictLT α] [DecidableLT α] [DecidableEq α] (s : Set α) :
+public theorem inter_empty_left {α} [LT α] [StrictLT α] [DecidableLT α] [DecidableEq α] (s : Set α) :
  Set.empty ∩ s = Set.empty
 := by
   cases s ; rename_i xs
   simp only [Inter.inter, intersect, List.inter, elts, List.elem_eq_mem, empty, List.filter_nil]
 
-theorem inter_empty_right {α} [LT α] [StrictLT α] [DecidableLT α] [DecidableEq α] (s : Set α) :
+public theorem inter_empty_right {α} [LT α] [StrictLT α] [DecidableLT α] [DecidableEq α] (s : Set α) :
  s ∩ Set.empty = Set.empty
 := by
   cases s ; rename_i xs
   simp only [Inter.inter, intersect, List.inter, elts, empty, List.elem_eq_mem, List.not_mem_nil,
     decide_false, mk.injEq, List.filter_eq_nil_iff, not_false_eq_true, implies_true, reduceCtorEq]
 
-theorem inter_self_eq {α} [LT α] [StrictLT α] [DecidableLT α] [DecidableEq α] (s : Set α) :
+public theorem inter_self_eq {α} [LT α] [StrictLT α] [DecidableLT α] [DecidableEq α] (s : Set α) :
  s ∩ s = s
 := by
   simp only [Inter.inter, intersect, List.inter, elts, List.elem_eq_mem]
@@ -428,7 +433,7 @@ theorem inter_self_eq {α} [LT α] [StrictLT α] [DecidableLT α] [DecidableEq �
     intro _ h
     simp only [h, implies_true]
 
-theorem intersects_def {α} [LT α] [StrictLT α] [DecidableLT α] [DecidableEq α] {s₁ s₂ : Set α} :
+public theorem intersects_def {α} [LT α] [StrictLT α] [DecidableLT α] [DecidableEq α] {s₁ s₂ : Set α} :
  s₁.intersects s₂ = ¬ (s₁ ∩ s₂).isEmpty
 := by
   simp only [Bool.not_eq_true, eq_iff_iff]
@@ -437,7 +442,7 @@ theorem intersects_def {α} [LT α] [StrictLT α] [DecidableLT α] [DecidableEq 
   case mp =>
     intro h
     replace ⟨x, h⟩ := h
-    by_contra hc
+    false_or_by_contra ; rename_i hc
     simp only [ne_eq, Bool.not_eq_false] at hc
     simp only [empty_iff_not_exists, not_exists] at hc
     specialize hc x
@@ -452,7 +457,7 @@ theorem intersects_def {α} [LT α] [StrictLT α] [DecidableLT α] [DecidableEq 
     rw [mem_inter_iff] at h
     exists x
 
-theorem intersects_iff_exists {α} [LT α] [StrictLT α] [DecidableLT α] [DecidableEq α] {s₁ s₂ : Set α} :
+public theorem intersects_iff_exists {α} [LT α] [StrictLT α] [DecidableLT α] [DecidableEq α] {s₁ s₂ : Set α} :
  s₁.intersects s₂ ↔ ∃ a, a ∈ s₁ ∧ a ∈ s₂
 := by
   constructor <;> intro h
@@ -465,12 +470,12 @@ theorem intersects_iff_exists {α} [LT α] [StrictLT α] [DecidableLT α] [Decid
     simp only [Set.intersects_def, Set.non_empty_iff_exists]
     exists a
 
-theorem union_wf [LT α] [DecidableLT α] [StrictLT α] (s₁ s₂ : Set α) :
+public theorem union_wf [LT α] [DecidableLT α] [StrictLT α] (s₁ s₂ : Set α) :
   WellFormed (s₁ ∪ s₂)
 := by
   simp only [Union.union, union, make_wf]
 
-theorem make_cons_eq_singleton_union [LT α] [DecidableLT α] [StrictLT α] (a : α) (L : List α) :
+public theorem make_cons_eq_singleton_union [LT α] [DecidableLT α] [StrictLT α] (a : α) (L : List α) :
   Set.make (a :: L) = Set.singleton a ∪ Set.make L := by
   rw [← eq_means_eqv (make_wf _) (union_wf _ _)]
   simp only [make, singleton, Union.union, union, elts]
@@ -478,7 +483,7 @@ theorem make_cons_eq_singleton_union [LT α] [DecidableLT α] [StrictLT α] (a :
   · apply List.Equiv.refl
   · simp [List.canonicalize_idempotent]
 
-theorem mem_union_iff_mem_or [LT α] [DecidableLT α] [StrictLT α] (s₁ s₂ : Set α) :
+public theorem mem_union_iff_mem_or [LT α] [DecidableLT α] [StrictLT α] (s₁ s₂ : Set α) :
   ∀ a, a ∈ s₁ ∪ s₂ ↔ (a ∈ s₁ ∨ a ∈ s₂)
 := by
   intro a
@@ -499,7 +504,7 @@ theorem mem_union_iff_mem_or [LT α] [DecidableLT α] [StrictLT α] (s₁ s₂ :
     · exact hc.left h
     · exact hc.right h
 
-theorem prop_union_iff_prop_and [LT α] [DecidableLT α] [StrictLT α] (p : α → Prop) (s₁ s₂ : Set α) :
+public theorem prop_union_iff_prop_and [LT α] [DecidableLT α] [StrictLT α] (p : α → Prop) (s₁ s₂ : Set α) :
   ((∀ a ∈ s₁, p a) ∧ (∀ a ∈ s₂, p a)) ↔ ∀ a ∈ (s₁ ∪ s₂), p a
 := by
   constructor <;> intro h₁
@@ -518,7 +523,7 @@ theorem prop_union_iff_prop_and [LT α] [DecidableLT α] [StrictLT α] (p : α �
       exact h₁
     }
 
-theorem union_comm [LT α] [DecidableLT α] [StrictLT α] (s₁ s₂ : Set α) :
+public theorem union_comm [LT α] [DecidableLT α] [StrictLT α] (s₁ s₂ : Set α) :
   s₁ ∪ s₂ = s₂ ∪ s₁
 := by
   simp only [Union.union, union, make, elts, mk.injEq]
@@ -526,7 +531,7 @@ theorem union_comm [LT α] [DecidableLT α] [StrictLT α] (s₁ s₂ : Set α) :
   simp only [List.Equiv, List.append_subset,
     List.subset_append_right, List.subset_append_left, and_self]
 
-theorem union_assoc [LT α] [DecidableLT α] [StrictLT α] (s₁ s₂ s₃ : Set α) :
+public theorem union_assoc [LT α] [DecidableLT α] [StrictLT α] (s₁ s₂ s₃ : Set α) :
   (s₁ ∪ s₂) ∪ s₃ = s₁ ∪ (s₂ ∪ s₃)
 := by
   rw [← eq_means_eqv (union_wf _ _) (union_wf _ _)]
@@ -546,20 +551,20 @@ theorem union_assoc [LT α] [DecidableLT α] [StrictLT α] (s₁ s₂ s₃ : Set
   simp only [List.append_assoc]
   exact List.append_right_equiv _ _ _ List.Equiv.refl
 
-theorem union_empty_right [LT α] [DecidableLT α] [StrictLT α] {s : Set α} :
+public theorem union_empty_right [LT α] [DecidableLT α] [StrictLT α] {s : Set α} :
   s.WellFormed → s ∪ Set.empty = s
 := by
   intro h
   simp only [WellFormed, toList, elts] at h
   simp only [Union.union, union, elts, empty, List.append_nil, ← h]
 
-theorem union_empty_left [LT α] [DecidableLT α] [StrictLT α] {s : Set α} :
+public theorem union_empty_left [LT α] [DecidableLT α] [StrictLT α] {s : Set α} :
   s.WellFormed → Set.empty ∪ s = s
 := by
   rw [union_comm]
   exact union_empty_right
 
-theorem union_idempotent [LT α] [DecidableLT α] [StrictLT α] {s : Set α} :
+public theorem union_idempotent [LT α] [DecidableLT α] [StrictLT α] {s : Set α} :
   s.WellFormed → s ∪ s = s
 := by
   intro h
@@ -570,7 +575,7 @@ theorem union_idempotent [LT α] [DecidableLT α] [StrictLT α] {s : Set α} :
 
 /-! ### subset -/
 
-theorem elts_subset_then_subset [LT α] [DecidableLT α] [StrictLT α] [DecidableEq α] {xs ys : List α} :
+public theorem elts_subset_then_subset [LT α] [DecidableLT α] [StrictLT α] [DecidableEq α] {xs ys : List α} :
   xs ⊆ ys → Set.make xs ⊆ Set.make ys
 := by
   simp only [Subset, List.Subset, subset, List.all_eq_true]
@@ -583,7 +588,7 @@ theorem elts_subset_then_subset [LT α] [DecidableLT α] [StrictLT α] [Decidabl
 /--
   Like `List.subset_def`, but lifted to Sets
 -/
-theorem subset_def [DecidableEq α] {s₁ s₂ : Set α} :
+public theorem subset_def [DecidableEq α] {s₁ s₂ : Set α} :
   s₁ ⊆ s₂ ↔ ∀ a, a ∈ s₁ → a ∈ s₂
 := by
   simp only [Subset, subset, List.all_eq_true]
@@ -597,7 +602,7 @@ theorem subset_def [DecidableEq α] {s₁ s₂ : Set α} :
     rw [contains_prop_bool_equiv]
     exact h₁ h₂
 
-theorem superset_empty_subset_empty [DecidableEq α] {s₁ s₂ : Set α} :
+public theorem superset_empty_subset_empty [DecidableEq α] {s₁ s₂ : Set α} :
   s₁ ⊆ s₂ → s₂.isEmpty → s₁.isEmpty
 := by
   repeat rw [Set.empty_iff_not_exists]
@@ -608,45 +613,45 @@ theorem superset_empty_subset_empty [DecidableEq α] {s₁ s₂ : Set α} :
   exists a
   exact h₁ a h₃
 
-theorem subset_iff_subset_elts [DecidableEq α] {s₁ s₂ : Set α} :
+public theorem subset_iff_subset_elts [DecidableEq α] {s₁ s₂ : Set α} :
   s₁ ⊆ s₂ ↔ s₁.elts ⊆ s₂.elts
 := by
   simp only [subset_def, elts, List.subset_def, in_list_iff_in_set]
 
-theorem subset_iff_eq [LT α] [DecidableLT α] [StrictLT α] [DecidableEq α] {s₁ s₂ : Set α} :
+public theorem subset_iff_eq [LT α] [DecidableLT α] [StrictLT α] [DecidableEq α] {s₁ s₂ : Set α} :
   WellFormed s₁ → WellFormed s₂ →
   ((s₁ ⊆ s₂ ∧ s₂ ⊆ s₁) ↔ s₁ = s₂)
 := by
   intro hw₁ hw₂
   simp only [← (eq_means_eqv hw₁ hw₂), elts, List.Equiv, subset_iff_subset_elts]
 
-theorem subset_trans [DecidableEq α] {s₁ s₂ s₃ : Set α} :
+public theorem subset_trans [DecidableEq α] {s₁ s₂ s₃ : Set α} :
   s₁ ⊆ s₂ → s₂ ⊆ s₃ → s₁ ⊆ s₃
 := by
   simp only [subset_def]
   intro h₁ h₂ a ha
   exact h₂ a (h₁ a ha)
 
-theorem subset_refl [DecidableEq α] {s : Set α} :
+public theorem subset_refl [DecidableEq α] {s : Set α} :
   s ⊆ s
 := by
   simp only [subset_def, imp_self, implies_true]
 
-theorem mem_subset_mem [DecidableEq α] {a : α} {s₁ s₂ : Set α} :
+public theorem mem_subset_mem [DecidableEq α] {a : α} {s₁ s₂ : Set α} :
   a ∈ s₁ → s₁ ⊆ s₂ → a ∈ s₂
 := by
   simp only [subset_def]
   intro h₁ h₂
   exact h₂ a h₁
 
-theorem subset_union [LT α] [DecidableLT α] [StrictLT α] [DecidableEq α] (s₁ s₂ : Set α) :
+public theorem subset_union [LT α] [DecidableLT α] [StrictLT α] [DecidableEq α] (s₁ s₂ : Set α) :
   s₁ ⊆ s₁ ∪ s₂
 := by
   simp only [subset_def, mem_union_iff_mem_or]
   intro a hin
   exact Or.inl hin
 
-theorem union_subset [LT α] [DecidableLT α] [StrictLT α] [DecidableEq α] {s₁ s₂ s₃ : Set α} :
+public theorem union_subset [LT α] [DecidableLT α] [StrictLT α] [DecidableEq α] {s₁ s₂ s₃ : Set α} :
   s₁ ∪ s₂ ⊆ s₃ ↔ s₁ ⊆ s₃ ∧ s₂ ⊆ s₃
 := by
   simp only [subset_def, mem_union_iff_mem_or]
@@ -665,7 +670,7 @@ theorem union_subset [LT α] [DecidableLT α] [StrictLT α] [DecidableEq α] {s�
     · exact h.left a hor
     · exact h.right a hor
 
-theorem union_subset_eq [LT α] [DecidableLT α] [StrictLT α] [DecidableEq α] {s₁ s₂ : Set α} :
+public theorem union_subset_eq [LT α] [DecidableLT α] [StrictLT α] [DecidableEq α] {s₁ s₂ : Set α} :
   s₂.WellFormed → s₁ ⊆ s₂ → s₁ ∪ s₂ = s₂
 := by
   intro h₁ h₂
@@ -675,7 +680,7 @@ theorem union_subset_eq [LT α] [DecidableLT α] [StrictLT α] [DecidableEq α] 
   · rw [union_comm]
     exact subset_union _ _
 
-theorem wellFormed_correct {α} [LT α] [StrictLT α] [DecidableLT α] {s : Set α} :
+public theorem wellFormed_correct {α} [LT α] [StrictLT α] [DecidableLT α] {s : Set α} :
   s.wellFormed = true ↔ s.WellFormed
 := by
   constructor
@@ -691,37 +696,37 @@ theorem wellFormed_correct {α} [LT α] [StrictLT α] [DecidableLT α] {s : Set 
 /-! ### map -/
 
 /-- Analogue of `List.mem_map` but for sets -/
-theorem mem_map [LT α] [DecidableLT α] [StrictLT α] [LT β] [DecidableLT β] [StrictLT β] (b : β) (f : α → β) (s : Set α) :
+public theorem mem_map [LT α] [DecidableLT α] [StrictLT α] [LT β] [DecidableLT β] [StrictLT β] (b : β) (f : α → β) (s : Set α) :
   b ∈ s.map f ↔ ∃ a ∈ s, f a = b
 := by
   simp [Set.map, ← Set.make_mem, Set.in_list_iff_in_set]
 
 /-! ### filter and differences -/
 
-theorem filter_wf [LT α] [DecidableLT α] [StrictLT α] (p : α → Bool) (s : Set α) :
+public theorem filter_wf [LT α] [DecidableLT α] [StrictLT α] (p : α → Bool) (s : Set α) :
   WellFormed s →
   WellFormed (s.filter p)
 := by
   simp only [Set.filter, wf_iff_sorted]
   apply List.filter_sortedBy
 
-theorem mem_filter [LT α] [DecidableLT α] [StrictLT α] (p : α → Bool) (s : Set α) (e : α):
+public theorem mem_filter [LT α] [DecidableLT α] [StrictLT α] (p : α → Bool) (s : Set α) (e : α):
   e ∈ s.filter p ↔ (e ∈ s ∧ p e)
 := by
   simp only [filter]
   rw [←in_list_iff_in_mk, ←in_list_iff_in_set]
   simp [List.mem_filter]
 
-theorem difference_wf [LT α] [DecidableLT α] [StrictLT α] [DecidableEq α] (s₁ s₂ : Set α) :
+public theorem difference_wf [LT α] [DecidableLT α] [StrictLT α] [DecidableEq α] (s₁ s₂ : Set α) :
   WellFormed s₁ →
   WellFormed (s₁.difference s₂)
 := by apply filter_wf
 
-theorem mem_difference [LT α] [DecidableLT α] [StrictLT α] [DecidableEq α] (s₁ s₂ : Set α) (e : α):
+public theorem mem_difference [LT α] [DecidableLT α] [StrictLT α] [DecidableEq α] (s₁ s₂ : Set α) (e : α):
   e ∈ s₁.difference s₂ ↔ (e ∈ s₁ ∧ e ∉ s₂)
 := by simp [difference, mem_filter, ←not_contains_prop_bool_equiv]
 
-theorem difference_subset [LT α] [DecidableLT α] [StrictLT α] [DecidableEq α] (s₁ s₂ : Set α) :
+public theorem difference_subset [LT α] [DecidableLT α] [StrictLT α] [DecidableEq α] (s₁ s₂ : Set α) :
   (s₁.difference s₂) ⊆ s₁
 := by
   rw [subset_def]
