cedar-lean/Cedar/Thm/Data/List.lean
@@ -14,6 +14,8 @@
  limitations under the License.
 -/
 
-import Cedar.Thm.Data.List.Basic
-import Cedar.Thm.Data.List.Canonical
-import Cedar.Thm.Data.List.Lemmas
+module
+
+public import Cedar.Thm.Data.List.Basic
+public import Cedar.Thm.Data.List.Canonical
+public import Cedar.Thm.Data.List.Lemmas
